refactor adding sections for abstrating the strength of assumptions

src/Rdf.v
@@ -7,232 +7,247 @@ From RDF Require Import Triple.
 
 Section Rdf.
 
-  Variable I B L: countType.
-  Let term:= (term I B L).
-  Let triple:= (triple I B L).
-  Let code_triple:= (@code_triple I B L).
-  Let decode_triple:= (@decode_triple I B L).
-  Let cancel_triple_encode := (@cancel_triple_encode I B L).
+  Record rdf_graph {I B L : Type}:= mkRdfGraph {
+                                       graph : seq triple
+                                     ; subject_in_IB : all (fun t => @is_in_ib I B L (subject t)) graph
+                                     ; predicate_in_I : all (fun t => @is_in_i I B L (predicate t)) graph
+                                     ; object_in_IBL : all (fun t => @is_in_ibl I B L (object t)) graph
+                                     }.
 
-  Record rdf_graph := mkRdfGraph {
-                         graph : seq triple
-                       ; subject_in_IB : all (fun t => is_in_ib (subject t)) graph
-                       ; predicate_in_I : all (fun t => is_in_i (predicate t)) graph
-                       ; object_in_IBL : all (fun t => is_in_ibl (object t)) graph
-                       }.
+  Section PolyRdf.
+    Variables I B L : Type.
+    
+    Definition terms (g : @rdf_graph I B L) : seq term :=
+      flatten (map (fun t => terms_triple t) (graph g)).
 
-  Definition eqb_rdf (g1 g2 : rdf_graph) : bool :=
-    (graph g1) == (graph g2).
+    Definition bnodes (g : @rdf_graph I B L) : seq term :=
+      filter (fun t => is_bnode t) (terms g).
+    
+    Definition add_sib (ts : seq triple) (pall : all (fun t => is_in_ib (subject t)) ts) (t : triple) : all (fun t => @is_in_ib I B L (subject t)) (t::ts).
+    Proof. induction (t::ts).
+           - apply all_nil.
+           - rewrite /=. apply /andP ; split. by case a=> /= _ _ _ -> _ _. apply IHl.
+    Qed.
 
-  Definition terms (g : rdf_graph) : seq term :=
-    flatten (map (fun t => terms_triple t) (graph g)).
+    Definition add_i (ts : seq triple) (pall : all (fun t => is_in_i (predicate t)) ts) (t : triple) : all (fun t => @is_in_i I B L (predicate t)) (t::ts).
+    Proof. induction (t::ts).
+           - apply all_nil.
+           - rewrite /=. apply /andP ; split. by case a=> /= _ _ _ _ -> _. apply IHl.
+    Qed.
 
-  Definition bnodes (g : rdf_graph) : seq term :=
-    filter (fun t => is_bnode t) (terms g).
-  (* Notation "x \in G" := (in_mem x (mem (terms G))) (only parsing) : bool_scope. *)
+    Definition add_ibl (ts : seq triple) (pall : all (fun t => is_in_ibl (object t)) ts) (t : triple) : all (fun t => @is_in_ibl I B L (object t)) (t::ts).
+    Proof. induction (t::ts).
+           - apply all_nil.
+           - rewrite /=. apply /andP ; split. by case a=> /= _ _ _ _ _ ->. apply IHl.
+    Qed.
 
-  Lemma eqb_rdf_refl (g : rdf_graph) : eqb_rdf g g.
-  Proof. by rewrite /eqb_rdf. Qed.
+    Definition add_triple (sg : option (@rdf_graph I B L)) (t : (@triple I B L)) : option (@rdf_graph I B L).
+    Proof. destruct sg as [g |].
+           - destruct g as [g' sib ip ibl].
+             exact (Some {|
+                        graph := t :: g' ;
+                        subject_in_IB := (@add_sib g' sib t) ;
+                        predicate_in_I := (@add_i g' ip t) ;
+                        object_in_IBL := (@add_ibl g' ibl t)
+                      |}).
+           - exact None.
+    Defined.
 
-  Lemma eqb_rdf_symm (g1 g2 : rdf_graph) : eqb_rdf g1 g2 = eqb_rdf g2 g1.
-  Proof. by rewrite /eqb_rdf. Qed.
+    Definition relabeling_seq_triple (μ : B -> B) (g : seq (@triple I B L)) : seq triple := map (relabeling_triple μ) g.
 
-  Lemma graph_inj : forall (g1 g2: rdf_graph),
-      eqb_rdf g1 g2 ->
-      g1 = g2.
-  Proof.
-    move=> [g1 sib1 pi1 oibl1] [g2 sib2 pi2 oibl2] /= /eqP /= geq.
-    subst. by f_equal; apply eq_irrelevance.
-  Qed.
 
-  Definition code_rdf (g : rdf_graph) :=
-    let (g',_,_,_) := g in
-    GenTree.Node 0 (map code_triple g').
+    Lemma relabeling_seq_triple_comp_P (g1 g2 : seq triple) (eqb : g1 = g2) (μ : B->B) :
+      relabeling_seq_triple μ g1 = relabeling_seq_triple μ g2. by rewrite eqb. Qed.
 
-  Definition add_sib (ts : seq triple) (pall : all (fun t => is_in_ib (subject t)) ts) (t : triple) : all (fun t => is_in_ib (subject t)) (t::ts).
-  Proof. induction (t::ts).
-         - apply all_nil.
-         - rewrite /=. apply /andP ; split. by case a=> /= _ _ _ -> _ _. apply IHl.
-  Qed.
+    Lemma relabeling_seq_triple_comp (μ1 μ2 : B -> B) (g : seq triple) : relabeling_seq_triple μ1 (relabeling_seq_triple μ2 g) = (relabeling_seq_triple μ1 \o (relabeling_seq_triple μ2)) g.
+    Proof. by []. Qed.
 
-  Definition add_i (ts : seq triple) (pall : all (fun t => is_in_i (predicate t)) ts) (t : triple) : all (fun t => is_in_i (predicate t)) (t::ts).
-  Proof. induction (t::ts).
-         - apply all_nil.
-         - rewrite /=. apply /andP ; split. by case a=> /= _ _ _ _ -> _. apply IHl.
-  Qed.
+    Lemma relabeling_seq_triple_preserves_subject_in_IB (g : seq triple) (μ : B -> B) :
+      all (fun t => @is_in_ib I B L (subject t)) g ->
+      all (fun t => @is_in_ib I B L (subject t)) (relabeling_seq_triple μ g).
+    Proof. induction g => [//| /=]. move=> /andP [sinh sint]. apply /andP. split. case a => [s p o /= sintt pint oint].
+           by rewrite relabeling_term_preserves_is_in_ib in sintt; apply sintt.
+           by apply IHg; apply sint.
+    Qed.
 
-  Definition add_ibl (ts : seq triple) (pall : all (fun t => is_in_ibl (object t)) ts) (t : triple) : all (fun t => is_in_ibl (object t)) (t::ts).
-  Proof. induction (t::ts).
-         - apply all_nil.
-         - rewrite /=. apply /andP ; split. by case a=> /= _ _ _ _ _ ->. apply IHl.
-  Qed.
+    Lemma relabeling_seq_triple_preserves_predicate_in_I (g : seq triple) (μ : B -> B) :
+      all (fun t => is_in_i (predicate t)) g ->
+      all (fun t => is_in_i (predicate t)) (relabeling_seq_triple μ g).
+    Proof. induction g => [//| /=]. move=> /andP [pinh pin]. apply /andP. split. case a => [s p o /= sintt pint oint].
+           by rewrite relabeling_term_preserves_is_in_i in pint; apply pint.
+           by apply IHg; apply pin.
+    Qed.
 
-  Definition add_triple (sg : option rdf_graph) (t : triple) : option rdf_graph.
-  Proof. destruct sg as [g |].
-         - destruct g as [g' sib ip ibl].
-           exact (Some {|
-                      graph := t :: g' ;
-                      subject_in_IB := (@add_sib g' sib t) ;
-                      predicate_in_I := (@add_i g' ip t) ;
-                      object_in_IBL := (@add_ibl g' ibl t)
-                    |}).
-         - exact None.
-  Defined.
+    Lemma relabeling_seq_triple_preserves_object_in_IBL (g : seq triple) (μ : B -> B) :
+      all (fun t => is_in_ibl (object t)) g ->
+      all (fun t => is_in_ibl (object t)) (relabeling_seq_triple μ g).
+    Proof. induction g => [//| /=]. move=> /andP [oinh ointt]. apply /andP. split. case a => [s p o /= sintt pint oint].
+           by rewrite relabeling_term_preserves_is_in_ibl in oint; apply oint.
+           by apply IHg; apply ointt.
+    Qed.
 
-  Definition decode_rdf (x : GenTree.tree nat) : option rdf_graph.
-  Proof. destruct x.
-         - exact None.
-         - destruct n as [| n'].
-           + induction l as [| t ts IHts].
-             * exact (Some (mkRdfGraph
-                              (all_nil (fun t => is_in_ib (subject t)))
-                              (all_nil (fun t => is_in_i (predicate t)))
-                              (all_nil (fun t => is_in_ibl (object t)))
-                     )).
-             * destruct (decode_triple t) as [t'|].
-               -- apply (@add_triple IHts t').
-               -- exact None.
-           + exact None.
-  Defined.
+    Lemma relabeling_seq_triple_id (g : seq triple) : @relabeling_seq_triple id g = g.
+    Proof. induction g => [//|]. rewrite /relabeling_seq_triple /=. f_equal.
+           by rewrite relabeling_triple_id.
+           rewrite /relabeling_seq_triple in IHg. exact IHg.
+    Qed.
 
-  Lemma forget_hd {T : Type} (t : T) (st : seq T) {p: T -> bool} (pall: all p (t::st)) : all p st.
-  Proof. revert pall=> /=. by move /andP=> [_ ->]. Qed.
+    Lemma relabeling_seq_triple_comp_simpl (g : seq triple) (μ12 μ23 : B -> B) :
+      relabeling_seq_triple (μ23 \o μ12) g = (@relabeling_seq_triple μ23 \o (relabeling_seq_triple μ12)) g.
+    Proof. rewrite /relabeling_seq_triple /=.
+           elim g => [//|h t iht] /=. rewrite relabeling_triple_comp /=. by f_equal; apply iht.
+    Qed.
 
-  Lemma cancel_rdf_encode : pcancel code_rdf decode_rdf.
-  Proof. case => g sib ii ibl. rewrite /code_rdf /decode_rdf.
-         induction g as [| t ts IHts].
-         - rewrite /=. f_equal. by apply graph_inj.
-         - rewrite /=.
-           have cant : decode_triple (code_triple t) = Some t. apply cancel_triple_encode.
-           rewrite cant. rewrite IHts.
-         - apply (forget_hd sib). apply (forget_hd ii). apply (forget_hd ibl).
-           move=> sib' ii' ibl'. rewrite /add_triple /=. f_equal. apply graph_inj. by rewrite /eqb_rdf.
-  Qed.
+    Lemma graph_inj : forall (g1 g2: rdf_graph),
+        @graph I B L g1 = graph g2 ->
+        g1 = g2.
+    Proof.
+      move=> [g1 sib1 pi1 oibl1] [g2 sib2 pi2 oibl2] /= geq. subst. 
+      by f_equal; apply eq_irrelevance.
+    Qed.
 
-  (* Definition rdf_eqP : Equality.axiom eqb_rdf. *)
-  (* Proof. rewrite /Equality.axiom => x y. *)
-  (*        apply: (iffP idP) => //= [| ->]; *)
-  (*                            case: x y=> [g1 sib1 pi1 oibl1] [g2 sib2 pi2 oibl2]. apply graph_inj. by apply eqb_rdf_refl. *)
-  (* Qed. *)
+    Lemma forget_hd {T : Type} (t : T) (st : seq T) {p: T -> bool} (pall: all p (t::st)) : all p st.
+    Proof. revert pall=> /=. by move /andP=> [_ ->]. Qed.
 
-  (* Definition rdf_le (g1 g2: rdf_graph) : bool := *)
-  (*   seqprod_with d triple *)
+    Definition relabeling (μ : B -> B) (g : rdf_graph): rdf_graph :=
+      let (g',siib,pii,oiibl) := g in
+      {|
+        graph := relabeling_seq_triple μ g';
+        subject_in_IB :=  relabeling_seq_triple_preserves_subject_in_IB μ siib;
+        predicate_in_I := relabeling_seq_triple_preserves_predicate_in_I μ pii;
+        object_in_IBL := relabeling_seq_triple_preserves_object_in_IBL μ oiibl
+      |}.
 
-  (* Canonical rdf_eqType := EqType rdf_graph (EqMixin rdf_eqP). *)
+    Lemma relabeling_id (g : rdf_graph) : relabeling id g = g.
+    Proof. apply graph_inj. case g=> g' sin pin oin /=.
+           by rewrite relabeling_seq_triple_id.
+    Qed.
 
-  (* Canonical rdf_porderType := POrderType <= rdf_graph (lePOrderMixin). *)
-  Definition rdf_eqMixin := PcanEqMixin cancel_rdf_encode.
-  Definition rdf_canChoiceMixin := PcanChoiceMixin cancel_rdf_encode.
-  Definition rdf_canCountMixin := PcanCountMixin cancel_rdf_encode.
+    Lemma relabeling_comp (g : rdf_graph) (μ12 μ23: B -> B) :
+      (relabeling μ23 \o (relabeling μ12)) g = relabeling (μ23 \o μ12) g.
+    Proof. 
+      induction g => [//]. rewrite /relabeling /=. apply graph_inj => /=.
+      by rewrite relabeling_seq_triple_comp_simpl.
+    Qed.
 
-  Canonical rdf_eqType := Eval hnf in EqType rdf_graph rdf_eqMixin.
-  Canonical rdf_choiceType := Eval hnf in ChoiceType rdf_graph rdf_canChoiceMixin.
-  Canonical rdf_countType := Eval hnf in CountType rdf_graph rdf_canCountMixin.
+    Lemma relabeling_seq_triple_ext (μ1 μ2 : B -> B) : μ1 =1 μ2 -> forall g : seq (@triple I B L), relabeling_seq_triple μ1 g = relabeling_seq_triple μ2 g.
+    Proof. move => μpqeq. elim=> [//|h t IHt] /=. rewrite IHt. f_equal. by apply relabeling_triple_ext. Qed.
 
-  Definition rdf_canPOrderMixin := PcanPOrderMixin (@pickleK rdf_countType).
-  Canonical rdf_POrderType := Eval hnf in POrderType tt rdf_graph rdf_canPOrderMixin.
+    Lemma relabeling_ext  (μ1 μ2 : B -> B) :  μ1 =1 μ2 -> forall g, relabeling μ1 g = relabeling μ2 g.
+    Proof. move=> μpweq g. induction g. apply /graph_inj => /=. by apply relabeling_seq_triple_ext. Qed.
 
-  Definition relabeling_seq_triple (μ : B -> B) (g : seq triple) : seq triple := map (relabeling_triple μ) g.
+    Lemma relabeling_comp_simpl (μ1 μ2 : B -> B) (g : rdf_graph) : relabeling μ1 (relabeling μ2 g) = relabeling (μ1 \o μ2) g.
+    Proof. by rewrite -relabeling_comp. Qed.
+  End PolyRdf.
 
-  Lemma relabeling_seq_triple_id (g : seq triple) : relabeling_seq_triple id g = g.
-  Proof. rewrite /relabeling_seq_triple. apply /eqP.
-         elim g => [//|h t /eqP iht] /=. rewrite relabeling_triple_id. by rewrite iht. Qed.
+  Section EqRdf.
+    Variables I B L : eqType.
+    
+    Definition eqb_rdf (g1 g2 : @rdf_graph I B L) : bool :=
+      (graph g1) == (graph g2).
+    Lemma eqb_rdf_refl (g : rdf_graph) : eqb_rdf g g.
+    Proof. by rewrite /eqb_rdf. Qed.
 
-  Lemma relabeling_seq_triple_comp_simpl (g : seq triple) (μ12 μ23 : B -> B) :
-    relabeling_seq_triple (μ23 \o μ12) g = (relabeling_seq_triple μ23 \o (relabeling_seq_triple μ12)) g.
-  Proof. rewrite /relabeling_seq_triple /=.
-         elim g => [//|h t iht] /=. rewrite relabeling_triple_comp /=. by f_equal; apply iht.
-  Qed.
+    Lemma eqb_rdf_symm (g1 g2 : rdf_graph) : eqb_rdf g1 g2 = eqb_rdf g2 g1.
+    Proof. by rewrite /eqb_rdf. Qed.
 
-  Lemma relabeling_seq_triple_comp_P (g1 g2 : seq triple) (eqb : g1 = g2) (μ : B->B) :
-    relabeling_seq_triple μ g1 = relabeling_seq_triple μ g2. by rewrite eqb. Qed.
+    Definition rdf_eqP : Equality.axiom eqb_rdf.
+    Proof. rewrite /Equality.axiom => x y.
+           apply: (iffP idP) => //= [| ->];
+                               case: x y=> [g1 sib1 pi1 oibl1] [g2 sib2 pi2 oibl2]. rewrite /eqb_rdf => /eqP /= geq. subst. by apply graph_inj. by apply eqb_rdf_refl.
+    Qed.
 
-  Lemma relabeling_seq_triple_comp (μ1 μ2 : B -> B) (g : seq triple) : relabeling_seq_triple μ1 (relabeling_seq_triple μ2 g) = (relabeling_seq_triple μ1 \o (relabeling_seq_triple μ2)) g.
-  Proof. by []. Qed. 
+    Canonical rdf_eqType := EqType rdf_graph (EqMixin rdf_eqP).
 
-  Lemma relabeling_seq_triple_preserves_subject_in_IB (g : seq triple) (μ : B -> B) :
-    all (fun t => is_in_ib (subject t)) g ->
-    all (fun t => is_in_ib (subject t)) (relabeling_seq_triple μ g).
-  Proof. move=> /allP sin. apply /allP => [[s p o /= sint pint oint]] => tg. by apply sint. 
-  Qed.
+    Lemma bijective_eqb_rdf mu nu g1 g2 : cancel mu nu -> eqb_rdf g1 (relabeling mu g2) ->  eqb_rdf g2 (relabeling nu g1).
+    Proof.
+      move=> cancel_mu_nu. rewrite /eqb_rdf => /eqP /graph_inj ->. 
+      rewrite relabeling_comp_simpl.
+      have /relabeling_ext-> : nu \o mu =1 id by [].
+      rewrite relabeling_id; exact: eqb_rdf_refl.
+    Qed.
 
-  Lemma relabeling_seq_triple_preserves_predicate_in_I (g : seq triple) (μ : B -> B) :
-    all (fun t => is_in_i (predicate t)) g ->
-    all (fun t => is_in_i (predicate t)) (relabeling_seq_triple μ g).
-  Proof. move=> /allP pin. apply /allP => [[s p o /= sint pint oint]] => tg. by apply pint.
-  Qed.
+  End EqRdf.
 
-  Lemma relabeling_seq_triple_preserves_object_in_IBL (g : seq triple) (μ : B -> B) :
-    all (fun t => is_in_ibl (object t)) g ->
-    all (fun t => is_in_ibl (object t)) (relabeling_seq_triple μ g).
-  Proof. move=> /allP oin. apply /allP => [[s p o /= sibt pibt oint]] => tg. by apply oint.
-  Qed.
+  Section CountRdf.
+    Variables I B L : countType.
 
-  Definition relabeling (μ : B -> B) (g : rdf_graph): rdf_graph :=
-    let (g',siib,pii,oiibl) := g in
-    {|
-      graph := relabeling_seq_triple μ g';
-      subject_in_IB :=  relabeling_seq_triple_preserves_subject_in_IB μ siib;
-      predicate_in_I := relabeling_seq_triple_preserves_predicate_in_I μ pii;
-      object_in_IBL := relabeling_seq_triple_preserves_object_in_IBL μ oiibl
-    |}.
+    Definition code_rdf (g : rdf_graph) :=
+      let (g',_,_,_) := g in
+      GenTree.Node 0 (map (@code_triple I B L) g').
 
-  Lemma relabeling_id (g : rdf_graph) : relabeling id g = g.
-  Proof. apply graph_inj. case g=> g' sin pin oin. rewrite /relabeling /= /eqP /eqb_rdf /=. by rewrite /eqP relabeling_seq_triple_id.
-  Qed.
+    Definition decode_rdf (x : GenTree.tree nat) : option (@rdf_graph I B L).
+    Proof. destruct x.
+           - exact None.
+           - destruct n as [| n'].
+             + induction l as [| t ts IHts].
+               * exact (Some (mkRdfGraph
+                                (all_nil (fun t => is_in_ib (subject t)))
+                                (all_nil (fun t => is_in_i (predicate t)))
+                                (all_nil (fun t => is_in_ibl (object t)))
+                       )).
+               * destruct (@decode_triple I B L t) as [t'|].
+                 -- apply (@add_triple I B L IHts t').
+                 -- exact None.
+             + exact None.
+    Defined.
 
-  Lemma relabeling_comp (g : rdf_graph) (μ12 μ23: B -> B) :
-    (relabeling μ23 \o (relabeling μ12)) g = relabeling (μ23 \o μ12) g.
-  Proof. apply graph_inj. rewrite /eqb_rdf. apply /eqP.
-         case g=> g' sin pin oin /=. by rewrite relabeling_seq_triple_comp_simpl.
-  Qed.
+    Lemma cancel_rdf_encode : pcancel code_rdf decode_rdf.
+    Proof. case => g sib ii ibl. rewrite /code_rdf /decode_rdf.
+           induction g as [| t ts IHts].
+           - rewrite /=. f_equal. by apply graph_inj.
+           - rewrite /=.
+             have cant : (@decode_triple I B L (code_triple t)) = Some t. apply cancel_triple_encode.
+             rewrite cant. rewrite IHts.
+           - apply (forget_hd sib). apply (forget_hd ii). apply (forget_hd ibl).
+             move=> sib' ii' ibl'. rewrite /add_triple /=. f_equal. apply graph_inj. by rewrite /eqb_rdf.
+    Qed.
 
-  Definition is_iso (g1 g2 : rdf_graph) (μ : B -> B) :=
-    (bijective μ) /\ eqb_rdf g1 (relabeling μ g2).
 
-  Definition iso (g1 g2 : rdf_graph):= exists (μ : B -> B),
-      is_iso g1 g2 μ.
+    (* Canonical rdf_porderType := POrderType <= rdf_graph (lePOrderMixin). *)
+    Definition rdf_canChoiceMixin := PcanChoiceMixin cancel_rdf_encode.
+    Definition rdf_canCountMixin := PcanCountMixin cancel_rdf_encode.
 
-  Lemma iso_refl (g : rdf_graph) : iso g g.
-  Proof. rewrite /iso /is_iso; exists id; split.
-         exists id => //.
-         by rewrite relabeling_id eqb_rdf_refl.
-  Qed.
+    Canonical rdf_choiceType := Eval hnf in ChoiceType rdf_graph rdf_canChoiceMixin.
+    Canonical rdf_countType := Eval hnf in CountType rdf_graph rdf_canCountMixin.
 
-  Lemma relabeling_seq_triple_ext (μ1 μ2 : B -> B) : μ1 =1 μ2 -> forall g, relabeling_seq_triple μ1 g = relabeling_seq_triple μ2 g.
-  Proof. move => μpqeq. elim=> [//|h t IHt] /=. rewrite IHt. f_equal. by apply relabeling_triple_ext. Qed.
+    Definition rdf_canPOrderMixin := PcanPOrderMixin (@pickleK rdf_countType).
+    Canonical rdf_POrderType := Eval hnf in POrderType tt rdf_graph rdf_canPOrderMixin.
 
-  Lemma relabeling_ext  (μ1 μ2 : B -> B) :  μ1 =1 μ2 -> forall g, relabeling μ1 g = relabeling μ2 g.
-  Proof. move=> μpweq g. apply /graph_inj. rewrite /eqb_rdf. case g. rewrite /= => gs _ _ _. apply /eqP. by apply relabeling_seq_triple_ext. Qed.
 
-  Lemma relabeling_comp_simpl (μ1 μ2 : B -> B) (g : rdf_graph) : relabeling μ1 (relabeling μ2 g) = relabeling (μ1 \o μ2) g.
-  Proof. by rewrite -relabeling_comp. Qed.
+    Definition is_iso (g1 g2 : @rdf_graph I B L) (μ : B -> B) :=
+      (bijective μ) /\ eqb_rdf g1 (relabeling μ g2).
 
-  Lemma bijective_eqb_rdf mu nu g1 g2 : cancel mu nu -> eqb_rdf g1 (relabeling mu g2) ->  eqb_rdf g2 (relabeling nu g1).
-  Proof.
-    move=> cancel_mu_nu /graph_inj->.
-    rewrite relabeling_comp_simpl.
-    have /relabeling_ext-> : nu \o mu =1 id by [].
-    rewrite relabeling_id; exact: eqb_rdf_refl.
-  Qed.
+    Definition iso (g1 g2 : rdf_graph):= exists (μ : B -> B),
+        is_iso g1 g2 μ.
 
-  Lemma iso_symm (g1 g2 : rdf_graph) :
-    iso g1 g2 <-> iso g2 g1.
-  Proof.
-    rewrite /iso /is_iso.
-    split; case=> mu [mu_bij heqb_rdf]; case: (mu_bij)=> [nu h1 h2];
-                                                       (exists nu; split; [exact: bij_can_bij h1 | exact: bijective_eqb_rdf heqb_rdf]).
-  Qed. 
+    Lemma iso_refl (g : rdf_graph) : iso g g.
+    Proof. rewrite /iso /is_iso; exists id; split.
+           exists id => //.
+           by rewrite relabeling_id eqb_rdf_refl.
+    Qed.
 
-  Lemma iso_trans (g1 g2 g3: rdf_graph) : iso g1 g2 -> iso g2 g3 -> iso g1 g3.
-  Proof. rewrite /iso /is_iso=> [[μ1 [bij1 /graph_inj eqb1]] [μ2 [bij2 /graph_inj eqb2]]].
-         exists (μ1 \o μ2). split. 
-         rewrite /=. apply bij_comp. apply bij1. apply bij2.
-         rewrite -relabeling_comp /= -eqb2 -eqb1. by apply eqb_rdf_refl.
-  Qed.
 
-  Definition isocanonical_mapping (M : rdf_graph -> rdf_graph) :=
-    forall (g : rdf_graph),
-      iso (M g) g /\ forall (h : rdf_graph), iso (M g) (M h) <-> iso g h.
+    Lemma iso_symm (g1 g2 : rdf_graph) :
+      iso g1 g2 <-> iso g2 g1.
+    Proof.
+      rewrite /iso /is_iso.
+      split; case=> mu [mu_bij heqb_rdf]; case: (mu_bij)=> [nu h1 h2];
+                                                         (exists nu; split; [exact: bij_can_bij h1 | exact: bijective_eqb_rdf heqb_rdf]).
+    Qed. 
+
+
+    Lemma iso_trans (g1 g2 g3: rdf_graph) : iso g1 g2 -> iso g2 g3 -> iso g1 g3.
+    Proof. rewrite /iso /is_iso /eqb_rdf => [[μ1 [bij1 /eqP /graph_inj eqb1]] [μ2 [bij2 /eqP /graph_inj eqb2]]].
+           exists (μ1 \o μ2). split. 
+           rewrite /=. apply bij_comp. apply bij1. apply bij2.
+           rewrite -relabeling_comp /= -eqb2 -eqb1. by apply eqb_rdf_refl.
+    Qed.
+
+    Definition isocanonical_mapping (M : rdf_graph -> rdf_graph) :=
+      forall (g : rdf_graph),
+        iso (M g) g /\ forall (h : rdf_graph), iso (M g) (M h) <-> iso g h.
+
+  End CountRdf.
 
 End Rdf.
