src/Term.v
@@ -10,103 +10,134 @@ Section Term.
 
   (* literals should be of Datatype type, is not important for the moment*)
   Open Scope order_scope.
-  Variable I B L: countType.
 
-  Inductive term : Type :=
+  Inductive term {I B L : Type} : Type :=
   | Iri (id: I) 
   | Lit (l : L) 
   | Bnode (name : B).
+  
+  Section Poly.
+    Variables I B L : Type.
+    
+    Definition is_lit (t : @term I B L) : bool :=
+      (match t with
+       | Lit _ => true
+       | _ => false
+       end).
 
-  Definition code_term (x : term) :=
-    match x with
-    | Iri id => GenTree.Node 0 (GenTree.Leaf (pickle id) :: nil)
-    | Lit l => GenTree.Node 1 (GenTree.Leaf (pickle l) :: nil)
-    | Bnode name => GenTree.Node 2 (GenTree.Leaf (pickle name) :: nil)
-    end.
+    Definition is_iri (t : @term I B L) : bool :=
+      (match t with
+       | Iri _ => true
+       | _ => false
+       end).
 
-  Definition decode_term (x : GenTree.tree nat) : option term :=
-    match x with
-    | GenTree.Node 0 (GenTree.Leaf id :: nil) => omap Iri (unpickle id)
-    | GenTree.Node 1 (GenTree.Leaf l :: nil) =>  omap Lit (unpickle l)
-    | GenTree.Node 2 (GenTree.Leaf name :: nil) => omap Bnode (unpickle name)
-    | _ => None
-    end.
+    Definition is_bnode (t : @term I B L) : bool :=
+      (match t with
+       | Bnode _ => true
+       | _ => false
+       end).
 
-  Lemma cancel_code_decode : pcancel code_term decode_term.
-  Proof. case => [id | l | name]; by rewrite /= pickleK. Qed.
+    Definition is_in_ib (t : @term I B L) : bool :=
+      is_iri t || is_bnode t.
 
-  Definition term_eqMixin := PcanEqMixin cancel_code_decode.
-  Definition term_canChoiceMixin := PcanChoiceMixin cancel_code_decode.
-  Definition term_canCountMixin := PcanCountMixin cancel_code_decode.
+    Definition is_in_i (t : @term I B L) : bool :=
+      is_iri t.
 
-  Canonical term_eqType := Eval hnf in EqType term term_eqMixin.
-  Canonical term_choiceType := Eval hnf in ChoiceType term term_canChoiceMixin.
-  Canonical term_countType := Eval hnf in CountType term term_canCountMixin.
+    Definition is_in_ibl (t : @term I B L) : bool :=
+      is_iri t || is_bnode t || is_lit t.
 
-  Definition term_canPOrderMixin := PcanPOrderMixin (@pickleK term_countType).
-  Canonical term_POrderType := Eval hnf in POrderType tt term term_canPOrderMixin.
 
-  Definition is_lit (t : term ): bool :=
-    (match t with
-     | Lit _ => true
-     | _ => false
-     end).
+    Definition relabeling_term (μ : B -> B) (t : (@term I B L)) : term :=
+      match t with
+      | Bnode name => Bnode (μ name)
+      | _ => t
+      end.
 
-  Definition is_iri (t : term ) : bool :=
-    (match t with
-     | Iri _ => true
-     | _ => false
-     end).
+    Lemma relabeling_term_id (t: term) : relabeling_term id t = t.
+    Proof. by case t. Qed.
 
-  Definition is_bnode (t : term ) : bool :=
-    (match t with
-     | Bnode _ => true
-     | _ => false
-     end).
+    Lemma relabeling_term_comp (t: term) (μ1 μ2 : B -> B) : relabeling_term (μ2 \o μ1) t = (relabeling_term μ2 \o (relabeling_term μ1)) t.
+    Proof. by case t. Qed.
 
-  Definition is_in_ib (t : term) : bool :=
-    is_iri t || is_bnode t.
+    Lemma relabeling_term_id_p_I (t : term) (p: is_iri t) : is_iri (relabeling_term id t).
+    Proof. by rewrite relabeling_term_id p. Qed.
 
-  Definition is_in_i (t : term) : bool :=
-    is_iri t.
+    Lemma relabeling_term_id_p_L (t : term) (p: is_lit t) : is_lit (relabeling_term id t).
+    Proof. by rewrite relabeling_term_id p. Qed.
 
-  Definition is_in_ibl (t : term) : bool :=
-    is_iri t || is_bnode t || is_lit t.
+    Lemma relabeling_term_id_p_B (t : term) (p: is_iri t) : is_iri (relabeling_term id t).
+    Proof. by rewrite relabeling_term_id p. Qed.
 
-  Definition relabeling_term (μ : B -> B) (t : term) : term :=
-    match t with
-    | Bnode name => Bnode (μ name)
-    | _ => t
-    end.
+    Lemma relabeling_term_preserves_is_in_ib (μ : B -> B) (t : term) :
+      is_in_ib t <-> is_in_ib (relabeling_term μ t).
+    Proof. by case t. Qed.
 
-  Lemma relabeling_term_id (t: term) : relabeling_term id t = t.
-  Proof. by case t. Qed.
+    Lemma relabeling_term_preserves_is_in_i (μ : B -> B) (t : term) :
+      is_in_i t <-> is_in_i (relabeling_term μ t).
+    Proof. by case t. Qed.
 
-  Lemma relabeling_term_comp (t: term) (μ1 μ2 : B -> B) : relabeling_term (μ2 \o μ1) t = (relabeling_term μ2 \o (relabeling_term μ1)) t.
-  Proof. by case t. Qed.
+    Lemma relabeling_term_preserves_is_in_ibl (μ : B -> B) (t : term) :
+      is_in_ibl t <-> is_in_ibl (relabeling_term μ t).
+    Proof. by case t. Qed.
 
-  Lemma relabeling_term_id_p_I (t : term) (p: is_iri t) : is_iri (relabeling_term id t).
-  Proof. by rewrite relabeling_term_id p. Qed.
+    Lemma relabeling_term_ext (μ1 μ2 : B -> B) : μ1 =1 μ2 -> forall t : @term I B L, relabeling_term μ1 t = relabeling_term μ2 t.
+    Proof. move => μpweq [//| // | b] /=. by rewrite μpweq. Qed.
 
-  Lemma relabeling_term_id_p_L (t : term) (p: is_lit t) : is_lit (relabeling_term id t).
-  Proof. by rewrite relabeling_term_id p. Qed.
+  End Poly.
+  Section EqTerm.
+    Variables I B L : eqType.
 
-  Lemma relabeling_term_id_p_B (t : term) (p: is_iri t) : is_iri (relabeling_term id t).
-  Proof. by rewrite relabeling_term_id p. Qed.
 
-  Lemma relabeling_term_ext (μ1 μ2 : B -> B) : μ1 =1 μ2 -> forall t, relabeling_term μ1 t = relabeling_term μ2 t.
-  Proof. move => μpweq [//| // | b] /=. by rewrite μpweq. Qed.
+    Definition eqb_term (t1 t2 : @term I B L) : bool :=
+      match t1, t2 with
+      | Iri i1, Iri i2 => i1 == i2
+      | Bnode b1, Bnode b2 => b1 == b2
+      | Lit l1, Lit l2 => l1 == l2
+      | _, _ => false
+      end.
 
-  Lemma relabeling_term_preserves_is_in_ib (μ : B -> B) (t : term) :
-    is_in_ib t <-> is_in_ib (relabeling_term μ t).
-  Proof. by case t. Qed.
+    Lemma term_eqP : Equality.axiom eqb_term.
+    Proof.
+      rewrite /Equality.axiom => x y.
+      apply: (iffP idP) => //= [| ->]; rewrite /eqb_term; last by case y.
+      by case: x y=> [i1|l1|b1] [i2|l2|b2] // => /eqP ->. 
+    Qed.
 
-  Lemma relabeling_term_preserves_is_in_i (μ : B -> B) (t : term) :
-    is_in_i t <-> is_in_i (relabeling_term μ t).
-  Proof. by case t. Qed.
+    Canonical term_eqType := EqType term (EqMixin term_eqP).
+  End EqTerm.
+  Section CountTerm.
+    Variable I B L: countType.
 
-  Lemma relabeling_term_preserves_is_in_ibl (μ : B -> B) (t : term) :
-    is_in_ibl t <-> is_in_ibl (relabeling_term μ t).
-  Proof. by case t. Qed.
+    Definition code_term (x : (@term I B L)) :=
+      match x with
+      | Iri id => GenTree.Node 0 (GenTree.Leaf (pickle id) :: nil)
+      | Lit l => GenTree.Node 1 (GenTree.Leaf (pickle l) :: nil)
+      | Bnode name => GenTree.Node 2 (GenTree.Leaf (pickle name) :: nil)
+      end.
+
+    Definition decode_term (x : GenTree.tree nat) : option (@term I B L) :=
+      match x with
+      | GenTree.Node 0 (GenTree.Leaf id :: nil) => omap Iri (unpickle id)
+      | GenTree.Node 1 (GenTree.Leaf l :: nil) =>  omap Lit (unpickle l)
+      | GenTree.Node 2 (GenTree.Leaf name :: nil) => omap Bnode (unpickle name)
+      | _ => None
+      end.
+
+    Lemma cancel_code_decode : pcancel code_term decode_term.
+    Proof. case => [id | l | name]; by rewrite /= pickleK. Qed.
+
+    (*   Definition term_eqMixin := PcanEqMixin cancel_code_decode. *)
+    Definition term_canChoiceMixin := PcanChoiceMixin cancel_code_decode.
+    Definition term_canCountMixin := PcanCountMixin cancel_code_decode.
+
+    (*   Canonical term_eqType := Eval hnf in EqType term term_eqMixin. *)
+    Canonical term_choiceType := Eval hnf in ChoiceType term term_canChoiceMixin.
+    Canonical term_countType := Eval hnf in CountType term term_canCountMixin.
+
+    Definition term_canPOrderMixin := PcanPOrderMixin (@pickleK term_countType).
+    Canonical term_POrderType := Eval hnf in POrderType tt term term_canPOrderMixin.
+
+  End CountTerm.
+
 
 End Term.
