src/Triple.v
@@ -5,94 +5,120 @@ Unset Printing Implicit Defensive.
 From RDF Require Import Term.
 
 Section Triple.
-  Variable I B L: countType.
-  Let term:= (term I B L).
-  Let is_iri:= (@is_iri I B L).
-  Let is_bnode:= (@is_bnode I B L).
-  Let is_lit:= (@is_lit I B L).
-  Let code_term:= (@code_term I B L).
-  Let decode_term:= (@decode_term I B L).
-
-  Record triple := mkTriple { subject : term
-                            ; predicate : term
-                            ; object: term
-                            ; subject_in_IB: is_in_ib subject
-                            ; predicate_in_I: is_in_i predicate
-                            ; object_in_IBL: is_in_ibl object
-                    }. 
-
-  Lemma triple_inj : forall (t1 t2: triple),
-      subject t1 = subject t2 ->
-      predicate t1 = predicate t2 ->
-      object t1 = object t2 ->
-      t1 = t2.
-  Proof. move=> [s1 p1 o1 sin1 pin1 oin1] [s2 p2 o2 sin2 pin2 oin2] /= seq peq oeq.
-         subst. by f_equal; apply eq_irrelevance.
-  Qed.
-
-  Definition code_triple (t : triple) :=
-    let (s,p,o,_,_,_) := t in
-    GenTree.Node 0 [:: (code_term s); (code_term p) ; (code_term o)].
-
-  Definition decode_triple (x : GenTree.tree nat) : option triple.
-  Proof. destruct x eqn:E.
-         - exact None.
-         - destruct n as [| n'].
-           + destruct l as [| s [| p [| o]]] eqn:size.
-             * exact None.
-             * exact None.
-             * exact None.
-             * destruct l0.
-               -- destruct (decode_term s) as [dst | ] eqn:ds;
-                    destruct (decode_term p) as [dpt | ] eqn:dp;
-                    destruct (decode_term o) as [ dot| ] eqn:do.
-                                                               destruct (is_in_ib dst) eqn:iib;
-                                                                 destruct (is_in_i dpt) eqn:ii;
-                                                                 destruct (is_in_ibl dot) eqn: ibl.
-
-                                                               ++ exact (Some (mkTriple iib ii ibl)).
-                                                               + all: exact None. 
-  Defined.
   
-  Lemma cancel_triple_encode : pcancel code_triple decode_triple.
-  Proof. case => s p o sib ii oibl. rewrite /code_triple /decode_triple.
-         have cant: forall (t : term), decode_term (code_term t) = Some t. apply cancel_code_decode.
-         rewrite /= !cant; destruct s; destruct p ; destruct o => //=.
-         all: by f_equal; apply triple_inj. 
-  Qed. 
-  
-  Definition triple_eqMixin := PcanEqMixin cancel_triple_encode.
-  Definition triple_canChoiceMixin := PcanChoiceMixin cancel_triple_encode.
-  Definition triple_canCountMixin := PcanCountMixin cancel_triple_encode.
+  Record triple {I B L : Type} := mkTriple { subject : @term I B L
+                                           ; predicate : @term I B L
+                                           ; object: @term I B L 
+                                           ; subject_in_IB: is_in_ib subject
+                                           ; predicate_in_I: is_in_i predicate
+                                           ; object_in_IBL: is_in_ibl object
+                                   }. 
+  Section PolyTriple.
+    Variables I B L : Type.
+    
+    Definition relabeling_triple (μ : B -> B) (t : @triple I B L) : @triple I B L :=
+      let (s,p,o,sin,pin,oin) := t in
+      mkTriple ((iffLR (relabeling_term_preserves_is_in_ib μ s)) sin)
+               ((iffLR (relabeling_term_preserves_is_in_i μ p)) pin)
+               ((iffLR (relabeling_term_preserves_is_in_ibl μ o)) oin).
 
-  Canonical triple_eqType := Eval hnf in EqType triple triple_eqMixin.
-  Canonical triple_choiceType := Eval hnf in ChoiceType triple triple_canChoiceMixin.
-  Canonical triple_countType := Eval hnf in CountType triple triple_canCountMixin.
+    Definition terms_triple (t : @triple I B L) : seq term :=
+      let (s,p,o,_,_,_) := t in
+      [:: s ; p ; o].
 
-  Definition triple_canPOrderMixin := PcanPOrderMixin (@pickleK triple_countType).
-  Canonical triple_POrderType := Eval hnf in POrderType tt triple triple_canPOrderMixin.
+    Definition bnodes_triple (t : @triple I B L) : seq (@term I B L) :=
+      filter (@is_bnode I B L) (terms_triple t).
 
-  Definition relabeling_triple (μ : B -> B) (t : triple) : triple :=
-    let (s,p,o,sin,pin,oin) := t in
-    mkTriple ((iffLR (relabeling_term_preserves_is_in_ib μ s)) sin)
-             ((iffLR (relabeling_term_preserves_is_in_i μ p)) pin)
-             ((iffLR (relabeling_term_preserves_is_in_ibl μ o)) oin).
+    Lemma triple_inj : forall (t1 t2: triple),
+        subject t1 = subject t2 ->
+        predicate t1 = predicate t2 ->
+        @object I B L t1 = @object I B L t2 ->
+        t1 = t2.
+    Proof. move=> [s1 p1 o1 sin1 pin1 oin1] [s2 p2 o2 sin2 pin2 oin2] /= seq peq oeq.
+           subst. by f_equal; apply eq_irrelevance.
+    Qed.
 
-  Lemma relabeling_triple_id (t : triple) : relabeling_triple id t = t.
-  Proof.
-    case t => [s p o sin pin oin] /=. apply triple_inj => /=; by apply relabeling_term_id. Qed.
+    Lemma relabeling_triple_id (t : triple) : @relabeling_triple id t = t.
+    Proof.
+      case t => [s p o sin pin oin] /=. apply triple_inj => /=; by apply relabeling_term_id. Qed.
 
-  Lemma relabeling_triple_comp (μ1 μ2 : B -> B) (t : triple) : relabeling_triple (μ2 \o μ1) t = (relabeling_triple μ2 \o (relabeling_triple μ1)) t.
-  Proof. case t=> [s p o sin pin oin] /=. apply triple_inj=> /=; by rewrite relabeling_term_comp. Qed.
+    Lemma relabeling_triple_comp (μ1 μ2 : B -> B) (t : triple) : relabeling_triple (μ2 \o μ1) t = (@relabeling_triple μ2 \o (relabeling_triple μ1)) t.
+    Proof. case t=> [s p o sin pin oin] /=. apply triple_inj=> /=; by rewrite relabeling_term_comp. Qed.
 
-  Lemma relabeling_triple_ext (μ1 μ2 : B -> B) : μ1 =1 μ2 -> forall t, relabeling_triple μ1 t = relabeling_triple μ2 t.
-  Proof. move => μpweq t. apply /triple_inj; case t => /= [s p o _ _ _]; by apply (relabeling_term_ext μpweq). Qed.
+    Lemma relabeling_triple_ext (μ1 μ2 : B -> B) : μ1 =1 μ2 -> forall t, relabeling_triple μ1 t = @relabeling_triple μ2 t.
+    Proof. move => μpweq t. apply /triple_inj; case t => /= [s p o _ _ _]; by apply (@relabeling_term_ext I B L μ1 μ2 μpweq). Qed.
 
-  Definition terms_triple (t : triple) : seq term :=
-    let (s,p,o,_,_,_) := t in
-    [:: s ; p ; o].
 
-  Definition bnodes_triple (t : triple) : seq term :=
-    filter is_bnode (terms_triple t).
+  End PolyTriple.
+
+  Section EqTriple.
+    Variable I B L : eqType.
+    
+    Definition eqb_triple  (t1 t2 : @triple I B L) : bool :=
+      ((subject t1) == (subject t2)) &&
+        ((predicate t1) == (predicate t2)) &&
+        ((object t1) == (object t2)).
+
+    Lemma triple_eqP : Equality.axiom eqb_triple.
+    Proof.
+      rewrite /Equality.axiom => x y.
+      apply: (iffP idP) => //= [| ->]; rewrite /eqb_triple; case: x y=> [s1 p1 o1 sin1 pin1 oin1] [s2 p2 o2 sin2 pin2 oin2] //=.
+      case/andP; case/andP=> /eqP eq_s/eqP eq_p/eqP eq_o.
+      apply: triple_inj; move=> //= {sin1 sin2 pin1 pin2 oin1 oin2}; by apply /eqP.
+      by rewrite !eq_refl //.
+    Qed.
+
+    Canonical triple_eqType := EqType triple (EqMixin triple_eqP).
+
+  End EqTriple.
+
+  Section CountTriple. 
+    Variables I B L : countType.
+
+    Definition code_triple (t : @triple I B L) :=
+      let (s,p,o,_,_,_) := t in
+      GenTree.Node 0 [:: (code_term s); (code_term p) ; (code_term o)].
+
+    Definition decode_triple (x : GenTree.tree nat) : option (@triple I B L).
+    Proof. destruct x eqn:E.
+           - exact None.
+           - destruct n as [| n'].
+             + destruct l as [| s [| p [| o]]] eqn:size.
+               * exact None.
+               * exact None.
+               * exact None.
+               * destruct l0.
+                 -- destruct (@decode_term I B L s) as [dst | ] eqn:ds;
+                      destruct (@decode_term I B L p) as [dpt | ] eqn:dp;
+                      destruct (@decode_term I B L o) as [ dot| ] eqn:do.
+                                                                        destruct (is_in_ib dst) eqn:iib;
+                                                                          destruct (is_in_i dpt) eqn:ii;
+                                                                          destruct (is_in_ibl dot) eqn: ibl.
+
+                                                                        ++ exact (Some (mkTriple iib ii ibl)).
+                                                                        + all: exact None. 
+    Defined.
+    
+    Lemma cancel_triple_encode : pcancel code_triple decode_triple.
+    Proof. case => s p o sib ii oibl. rewrite /code_triple /decode_triple.
+           have cant: forall (t : term), @decode_term I B L (code_term t) = Some t. apply cancel_code_decode.
+           rewrite /= !cant; destruct s; destruct p ; destruct o => //=.
+           all: by f_equal; apply triple_inj. 
+    Qed. 
+    
+    (*   Definition triple_eqMixin := PcanEqMixin cancel_triple_encode. *)
+    Definition triple_canChoiceMixin := PcanChoiceMixin cancel_triple_encode.
+    Definition triple_canCountMixin := PcanCountMixin cancel_triple_encode.
+
+    (*   Canonical triple_eqType := Eval hnf in EqType triple triple_eqMixin. *)
+    Canonical triple_choiceType := Eval hnf in ChoiceType triple triple_canChoiceMixin.
+    Canonical triple_countType := Eval hnf in CountType triple triple_canCountMixin.
+
+    Definition triple_canPOrderMixin := PcanPOrderMixin (@pickleK triple_countType).
+    Canonical triple_POrderType := Eval hnf in POrderType tt triple triple_canPOrderMixin.
+
+
+  End CountTriple.
+
 
 End Triple.
